Progress towards Limited Equivocation projections result

VLSM/Equivocators/Composition/LimitedEquivocation/LimitedEquivocation.v
@@ -13,6 +13,7 @@ From CasperCBC
     VLSM.Equivocators.Common VLSM.Equivocators.Projections
     VLSM.Equivocators.MessageProperties
     VLSM.Equivocators.Composition.Common
+    VLSM.Equivocators.Composition.Projections
     VLSM.DependentMessages
     .
 
@@ -34,8 +35,8 @@ Context {message : Type}
   (equivocator_IM := equivocator_IM IM)
   (equivocator_descriptors_update := equivocator_descriptors_update IM)
   (proper_equivocator_descriptors := proper_equivocator_descriptors IM)
+  (sender : message -> option index)
   {Hmeasurable : Measurable index}
-  (equivocating : set index)
   {reachable_threshold : ReachableThreshold index}
   .
 
@@ -57,7 +58,6 @@ End limited_state_equivocation.
 
 Section limited_state_equivocation_with_full_node.
 
-
 Context {message : Type}
   {index : Type}
   {IndEqDec : EqDecision index}
@@ -72,14 +72,12 @@ Context {message : Type}
   (equivocator_IM := equivocator_IM IM)
   (equivocator_descriptors_update := equivocator_descriptors_update IM)
   (proper_equivocator_descriptors := proper_equivocator_descriptors IM)
-  {Hmeasurable : Measurable index}
   (equivocating : set index)
-  {reachable_threshold : ReachableThreshold index}
-  {validator : Type}
-  (A : validator -> index)
-  (sender : message -> option validator)
+  (sender : message -> option index)
   (Hbr : forall i, has_been_received_capability (IM i))
-  {Hdm : DependentMessages sender A IM Hbs Hbr}
+  {Hdm : DependentMessages sender (fun i => i) IM Hbs Hbr}
+  {Hmeasurable : Measurable index}
+  {reachable_threshold : ReachableThreshold index}
   .
 
 Existing Instance Hdm.
@@ -105,6 +103,9 @@ Definition full_node_equivocators_limited_equivocation_constraint
   full_node_equivocators_constraint l som /\
   equivocators_limited_equivocations_constraint IM Hbs finite_index l som.
 
+Definition full_node_equivocators_limited_equivocation_vlsm : VLSM message :=
+  composite_vlsm equivocator_IM full_node_equivocators_limited_equivocation_constraint.
+
 End limited_state_equivocation_with_full_node.
 
 Section limited_message_equivocation.
@@ -113,11 +114,9 @@ Context
   {message : Type}
   {index : Type}
   {IndEqDec : EqDecision index}
-  (index_listing : list index)
+  {index_listing : list index}
   (finite_index : Listing index_listing)
-  {validator : Type}
-  {ValMeasurable : Measurable validator}
-  {ValEqDec : EqDecision validator}
+  {ValMeasurable : Measurable index}
   (IM : index -> VLSM message)
   (Hbs : forall i, has_been_sent_capability (IM i))
   (Hbr : forall i, has_been_received_capability (IM i))
@@ -127,32 +126,52 @@ Context
   (X_has_been_sent_capability : has_been_sent_capability X := composite_has_been_sent_capability IM (free_constraint IM) finite_index Hbs)
   (X_has_been_received_capability : has_been_received_capability X := composite_has_been_received_capability IM (free_constraint IM) finite_index Hbr)
   (X_has_been_observed_capability : has_been_observed_capability X := has_been_observed_capability_from_sent_received X)
-  (A : validator -> index)
-  (sender : message -> option validator)
-  (globally_known_equivocators : composite_state IM -> set validator)
-  {Hdm : DependentMessages sender A IM Hbs Hbr}
-  {reachable_threshold : ReachableThreshold validator}
+  (sender : message -> option index)
+  (globally_known_equivocators : composite_state IM -> set index)
+  {Hdm : DependentMessages sender (fun i => i) IM Hbs Hbr}
+  {reachable_threshold : ReachableThreshold index}
   .
 
 Existing Instance X_has_been_observed_capability.
 
-Definition known_equivocators_transition_no_equiv_prop : Prop :=
-  forall
-    l s iom s' oom,
-    composite_transition IM l (s, iom) = (s', oom) ->
-    no_additional_equivocations_constraint X l (s, iom) ->
-    set_eq (globally_known_equivocators s') (globally_known_equivocators s).
+Class known_equivocators_capability :=
+  { known_equivocators_nodup :
+    forall s, NoDup (globally_known_equivocators s)
+  ; known_equivocators_initial_state :
+    forall s,
+      composite_initial_state_prop IM s ->
+      globally_known_equivocators s = []
+  ; known_equivocators_transition_no_equiv : 
+    forall
+      l s iom s' oom,
+      composite_transition IM l (s, iom) = (s', oom) ->
+      no_additional_equivocations_constraint X l (s, iom) ->
+      set_eq (globally_known_equivocators s') (globally_known_equivocators s)
+  ; known_equivocators_transition_equiv :
+    forall
+      l s im s' oom v,
+      composite_transition IM l (s, Some im) = (s', oom) ->
+      ~ no_additional_equivocations_constraint X l (s, Some im) ->
+      dependent_messages_global_full_node_condition finite_index s im ->
+      sender im = Some v ->
+      set_eq
+        (globally_known_equivocators s')
+        (set_add decide_eq v (globally_known_equivocators s))
+  }.
 
-Definition known_equivocators_transition_equiv_prop : Prop :=
-  forall
-    l s im s' oom v,
-    composite_transition IM l (s, Some im) = (s', oom) ->
-    ~ no_additional_equivocations_constraint X l (s, Some im) ->
-    dependent_messages_global_full_node_condition finite_index s im ->
-    sender im = Some v ->
-    set_eq
-      (globally_known_equivocators s')
-      (set_add decide_eq v (globally_known_equivocators s)).
+Context
+  {Hknown_equivocators : known_equivocators_capability}
+  .
+
+Lemma composite_transition_None_known_equivocators
+  l s s' oom
+  (Ht: composite_transition IM l (s, None) = (s', oom))
+  : set_eq (globally_known_equivocators s') (globally_known_equivocators s).
+Proof.
+  specialize (known_equivocators_transition_no_equiv _ _ _ _ _ Ht) as Heqv.
+  spec Heqv. { exact I. }
+  assumption.
+Qed.
 
 Definition globally_known_equivocators_weight
   (s : composite_state IM)
@@ -160,12 +179,537 @@ Definition globally_known_equivocators_weight
   :=
   sum_weights (globally_known_equivocators s).
 
+Lemma initial_state_equivocators_weight
+  (s : composite_state IM)
+  (Hs : composite_initial_state_prop IM s)
+  : globally_known_equivocators_weight s = 0%R.
+Proof.
+  apply known_equivocators_initial_state in Hs.
+  unfold globally_known_equivocators_weight.
+  rewrite Hs. reflexivity.
+Qed.
+
+Lemma composite_transition_None_equivocators_weight
+  l s s' oom
+  : composite_transition IM l (s, None) = (s', oom) ->
+    globally_known_equivocators_weight s' = globally_known_equivocators_weight s.
+Proof.
+  intro Ht.
+  specialize (composite_transition_None_known_equivocators _ _ _ _ Ht) as Heqv.
+  apply
+    (set_eq_nodup_sum_weight_eq
+      (globally_known_equivocators s')
+      (globally_known_equivocators s)
+    )
+  ; [..|assumption]
+  ; apply known_equivocators_nodup.
+Qed.
+
 Definition full_node_limited_equivocation_constraint
   (l : composite_label IM)
   (som : composite_state IM * option message)
   :=
   dependent_messages_local_full_node_constraint l som /\
   let (s', om') := composite_transition IM l som in
-  (globally_known_equivocators_weight s' < proj1_sig threshold)%R.
+  (globally_known_equivocators_weight s' <= proj1_sig threshold)%R.
+
+
+Definition full_node_limited_equivocation_vlsm_composition
+  :=
+  composite_vlsm IM full_node_limited_equivocation_constraint.
+
+Lemma full_node_limited_equivocation_protocol_state_weight s
+  : protocol_state_prop full_node_limited_equivocation_vlsm_composition s ->
+    (globally_known_equivocators_weight s <= proj1_sig threshold)%R.
+Proof.
+  intro Hs.
+  induction Hs using protocol_state_prop_ind.
+  - rewrite (initial_state_equivocators_weight s Hs).
+    destruct threshold. intuition.
+  - destruct Ht as [[Hs [Hom [Hv [Hc Hw]]]] Ht].
+    unfold transition in Ht. simpl in Ht.
+    simpl in Hw.
+    rewrite Ht in Hw.
+    assumption.
+Qed.
 
 End limited_message_equivocation.
+
+Section limited_equivocation_state_to_message.
+
+(** ** From composition of equivocators to composition of simple nodes
+
+In this section we show that the projection of [protocol_trace]s of a
+composition of equivocators with a fixed equivocation constraint are
+[protocol_trace]s for the composition of nodes with a similar fixed
+equivocation constraint.
+*)
+
+Context
+  {message : Type}
+  `{EqDecision message}
+  (index : Type)
+  {IndEqDec : EqDecision index}
+  (IM : index -> VLSM message)
+  (Hbs : forall i : index, has_been_sent_capability (IM i))
+  (Hbr : forall i : index, has_been_received_capability (IM i))
+  (i0 : Inhabited index)
+  (*equivocating : set index)
+  (Hi0_equiv : equivocating <> []*)
+  (* i0 : Inhabited index := @SubProjectionTraces.i0 index equivocating Hi0_equiv *)
+  {index_listing : list index}
+  (finite_index : Listing index_listing)
+  {ValMeasurable : Measurable index}
+  (sender : message -> option index)
+  (globally_known_equivocators : composite_state IM -> set index)
+  {Hdm : DependentMessages sender (fun i => i) IM Hbs Hbr}
+  {Hknown_equivocators : known_equivocators_capability finite_index IM Hbs Hbr i0 sender globally_known_equivocators}
+  {reachable_threshold : ReachableThreshold index}
+  (XE : VLSM message := full_node_equivocators_limited_equivocation_vlsm IM Hbs finite_index sender Hbr)
+  (X : VLSM message := full_node_limited_equivocation_vlsm_composition IM Hbs Hbr i0 sender globally_known_equivocators)
+  (equivocators_free_Hbs := composite_has_been_sent_capability (equivocator_IM IM) (free_constraint (equivocator_IM IM)) finite_index (equivocator_Hbs IM Hbs))
+  (FreeE : VLSM message := free_composite_vlsm (equivocator_IM IM))
+  (FreeE_has_been_sent_capability : has_been_sent_capability FreeE := composite_has_been_sent_capability (equivocator_IM IM) (free_constraint (equivocator_IM IM)) finite_index (equivocator_Hbs IM Hbs))
+  (Hdec_init : forall i, vdecidable_initial_messages_prop (IM i))
+  (comopsite_initial_decidable := composite_decidable_initial_message IM finite_index Hdec_init)
+  (Free := free_composite_vlsm IM)
+  (Free_has_been_sent_capability : has_been_sent_capability Free := composite_has_been_sent_capability IM (free_constraint IM) finite_index Hbs)
+  (Free_has_been_received_capability : has_been_received_capability Free := composite_has_been_received_capability IM (free_constraint IM) finite_index Hbr)
+  (Free_has_been_observed_capability : has_been_observed_capability Free := has_been_observed_capability_from_sent_received Free)
+  (Free_no_additional_equivocation_decidable := no_additional_equivocations_dec Free comopsite_initial_decidable)
+  (* index_equivocating_prop : index -> Prop := sub_index_prop equivocating *)
+  (* equivocating_index : Type := sub_index equivocating *)
+  (* equivocating_i0 : Inhabited equivocating_index := sub_index_i0 equivocating Hi0_equiv *)
+  (* equivocating_IM := sub_IM IM equivocating *)
+  (* equivocating_index_eq_dec : EqDecision equivocating_index := sub_index_eq_dec equivocating *)
+  (* free_equivocating_vlsm_composition : VLSM message := free_composite_vlsm equivocating_IM *)
+  (* sub_equivocator_IM := sub_IM (equivocator_IM IM) equivocating *)
+  .
+
+
+(**
+Inclusion in the free composition
+*)
+Lemma equivocators_limited_equivocations_vlsm_incl_free
+  : VLSM_incl XE (free_composite_vlsm (equivocator_IM IM)).
+Proof.
+  apply constraint_subsumption_incl.
+  intros l som H. exact I.
+Qed.
+
+(**
+Inclusion in the composition of equivocators with no message equivocation
+(no restriction on state equivocation).
+*)
+Lemma equivocators_limited_equivocations_vlsm_incl_no_equivocations
+  : VLSM_incl XE (equivocators_no_equivocations_vlsm IM Hbs finite_index).
+Proof.
+  apply constraint_subsumption_incl.
+  intros l som H. apply H.
+Qed.
+
+
+Existing Instance i0.
+
+
+Lemma limited_equivocators_initial_state_project
+  (es : vstate XE)
+  (Hes : vinitial_state_prop XE es)
+  (eqv_descriptors : equivocator_descriptors IM)
+  (Heqv : proper_equivocator_descriptors IM eqv_descriptors es)
+  : vinitial_state_prop X (equivocators_state_project IM eqv_descriptors es).
+Proof.
+  intro eqv. specialize (Hes eqv).
+  unfold equivocator_IM in Hes.
+  unfold equivocators_state_project.
+  specialize (Heqv eqv).
+  destruct (eqv_descriptors eqv) as [sn | i fi]; [assumption|].
+  destruct Hes as [Hzero Hes].
+  destruct (es eqv) as (n, bs). simpl in Heqv.
+  destruct (le_lt_dec (S n) i); [lia|].
+  simpl in *.
+  subst. assert (Hi: i = 0) by lia. subst.
+  assumption.
+Qed.
+
+Lemma fixed_equivocators_initial_message
+  (m : message)
+  (Hem : vinitial_message_prop XE m)
+  : vinitial_message_prop X m.
+Proof.
+  destruct Hem as [eqv [emi Hem]].
+  exists eqv.
+  unfold equivocator_IM in emi.
+  exists emi. assumption.
+Qed.
+
+
+(*
+
+(**
+[proper_equivocator_descriptors] strengthen for fixed-equivocation.
+We require that if the index is not equivocating, than the corresponding
+descriptor is a [zero_descriptor].
+*)
+Definition proper_fixed_equivocator_descriptors
+  (eqv_descriptors : equivocator_descriptors IM)
+  (s : state)
+  : Prop
+  := proper_equivocator_descriptors IM eqv_descriptors s /\
+    forall i, ~In i equivocating -> eqv_descriptors i = Existing _ 0 false.
+
+*)
+
+(**
+[not_equivocating_equivocator_descriptors] satisfy the
+[proper_equivocator_descriptors] property.
+*)
+Lemma not_equivocating_equivocatos_descriptors_proper
+  (s : composite_state (equivocator_IM IM))
+  (Hs : protocol_state_prop XE s)
+  (eqv_descriptors : equivocator_descriptors IM)
+  (Heqv_descriptors : not_equivocating_equivocator_descriptors IM eqv_descriptors s)
+  : proper_equivocator_descriptors IM eqv_descriptors s.
+Proof.
+  apply not_equivocating_equivocator_descriptors_proper. assumption.
+Qed.
+
+(**
+Projections of (valid) traces of the composition of equivocators preserve
+[proper_equivocator_descriptors].
+*)
+Lemma equivocators_trace_project_preserves_proper_equivocator_descriptors
+  (is : composite_state (equivocator_IM IM))
+  (tr : list (composite_transition_item (equivocator_IM IM)))
+  (Htr : finite_protocol_trace_from (pre_loaded_with_all_messages_vlsm FreeE) is tr)
+  (s := last (map destination tr) is)
+  (descriptors : equivocator_descriptors IM)
+  (idescriptors : equivocator_descriptors IM)
+  (trX : list (composite_transition_item IM))
+  (HtrX : equivocators_trace_project IM descriptors tr = Some (trX, idescriptors))
+  : proper_equivocator_descriptors IM descriptors s -> proper_equivocator_descriptors IM idescriptors is.
+Proof.
+  apply (preloaded_equivocators_protocol_trace_project_proper_initial IM
+    _ _ Htr _ _ _ HtrX).
+Qed.
+
+Existing Instance equivocators_free_Hbs.
+Existing Instance Free_has_been_observed_capability.
+Existing Instance Free_has_been_sent_capability.
+
+(**
+This is a property of the [fixed_equivocation_constraint] which also
+trivially holds for the free constraint.  This property is sufficient for
+proving the [_equivocators_protocol_trace_project] lemma,
+which lets that lemma be used for both the composition of equivocators with
+fixed state-equivocation and the free composition.
+
+It basically says that if a message has_been_sent for a state of the
+composition of equivocators with no-message equivocations and fixed
+state-equivocations, then any of its projections should be allowed to receive it.
+*)
+Definition constraint_has_been_sent_prop
+  (constraint : composite_label IM -> composite_state IM * option message -> Prop)
+  : Prop :=
+  forall
+    (s : composite_state (equivocator_IM IM))
+    (Hs : protocol_state_prop XE s)
+    (descriptors : equivocator_descriptors IM)
+    (Hdescriptors : proper_equivocator_descriptors IM descriptors s)
+    (sX := @equivocators_state_project _ _ IndEqDec IM i0 descriptors s)
+    (m: message)
+    (Hm : has_been_sent FreeE s m)
+    l,
+  constraint l (sX, Some m).
+
+
+(**
+Generic proof that the projection of a trace of the composition of equivocators
+with no message equivocation and fixed state equivocation is protocol w.r.t.
+the composition of the regular nodes constrained by any constraint satisfying
+several properties, including the [constraint_has_been_sent_prop]erty.
+
+The proof proceeds by well founded induction on the length of the trace,
+performing an analysis on the final transition item of the trace.
+
+It uses the fact that the trace hase no message equivocation to extract a
+subtrace producing the message being received at the last transition and
+proves that it's a protocol message for the destination machine by using
+the induction hypothesis (that is why well-founded induction is used rather
+than a simpler induction principle).
+
+The constraint satisfaction for the projection of the final transition is
+for now assumes as hypothesis @Hconstraint_hbs@.
+*)
+Lemma _equivocators_protocol_trace_project
+  (final_descriptors : equivocator_descriptors IM)
+  (is : composite_state (equivocator_IM IM))
+  (tr : list (composite_transition_item (equivocator_IM IM)))
+  (final_state := finite_trace_last is tr)
+  (Hproper : proper_equivocator_descriptors IM final_descriptors final_state)
+  (Htr : finite_protocol_trace XE is tr)
+  (constraint : composite_label IM -> composite_state IM * option message -> Prop)
+  (X' := composite_vlsm IM constraint)
+  (HconstraintNone : forall l s, protocol_state_prop X' s -> constraint l (s, None))
+  (Hconstraintinitial : forall l s m, protocol_state_prop X' s -> vinitial_message_prop FreeE m -> constraint l (s, Some m))
+  (Hconstraint_hbs :  constraint_has_been_sent_prop constraint)
+  : exists
+    (trX : list (composite_transition_item IM))
+    (initial_descriptors : equivocator_descriptors IM)
+    (isX := equivocators_state_project IM initial_descriptors is)
+    (final_stateX := finite_trace_last isX trX),
+    proper_equivocator_descriptors IM initial_descriptors is /\
+    equivocators_trace_project IM final_descriptors tr = Some (trX, initial_descriptors) /\
+    equivocators_state_project IM final_descriptors final_state = final_stateX /\
+    finite_protocol_trace X' isX trX.
+Proof.
+  remember (length tr) as len_tr.
+  generalize dependent final_descriptors. generalize dependent tr.
+  induction len_tr using (well_founded_induction Wf_nat.lt_wf); intros.
+  subst len_tr.
+  destruct_list_last tr tr' lst Htr_lst.
+  - clear H. subst. unfold final_state in *. exists [], final_descriptors.
+    split; [assumption|]. split; [reflexivity|]. split; [reflexivity|].
+    remember (equivocators_state_project IM final_descriptors is) as isx.
+    cut (vinitial_state_prop X' isx).
+    { intro. split; [|assumption]. constructor.
+      apply protocol_state_prop_iff. left.
+      exists (exist _ _ H). reflexivity.
+    }
+    subst.
+    apply limited_equivocators_initial_state_project; [|apply Hproper].
+    apply Htr.
+  - specialize (H (length tr')) as H'.
+    spec H'. { rewrite app_length. simpl. lia. }
+    destruct Htr as [Htr Hinit].
+    apply finite_protocol_trace_from_app_iff in Htr.
+    destruct Htr as [Htr Hlst].
+    specialize (H' tr' (conj Htr Hinit) eq_refl).
+    specialize (equivocators_transition_item_project_proper_characterization IM final_descriptors lst) as Hproperx.
+    specialize
+      (equivocators_transition_item_project_preserves_zero_descriptors IM final_descriptors lst)
+      as Hzero.
+    unfold final_state in Hproper.
+    rewrite Htr_lst, finite_trace_last_is_last in Hproper.
+    spec Hproperx Hproper.
+    destruct Hproperx as [oitem [final_descriptors' [Hprojectx [Hitemx Hproperx]]]].
+    specialize (Hproperx (finite_trace_last is tr')).
+    unfold equivocators_trace_project.
+    rewrite fold_right_app.
+    match goal with
+    |- context [fold_right _ ?fld _] => remember fld as foldx
+    end.
+    simpl in Heqfoldx.
+    rewrite Hprojectx in Heqfoldx.
+    apply first_transition_valid in Hlst. destruct lst as (l, iom, s, oom). simpl in *.
+    destruct Hlst as [[Hs [Hiom [Hv Hc]]] Ht].
+    specialize (Hzero oitem final_descriptors' _ Ht Hv Hprojectx).
+    specialize (Hproperx Hv Ht).
+    destruct Hproperx as [Hproper' Hx].
+    (*
+    assert (Hproper' : proper_fixed_equivocator_descriptors final_descriptors' (last (map destination tr') is)).
+    { split; [assumption|].
+      intros i Hi. apply Hzero. clear Hzero. destruct Hproper as [_ Hzero].
+      apply Hzero. assumption.
+    }
+    clear _Hproper' Hzero.
+    *)
+    specialize (H' _ Hproper').
+    destruct H' as [trX' [initial_descriptors [_ [Htr_project [Hstate_project HtrX']]]]].
+    assert
+      (Htr' : finite_protocol_trace FreeE is tr').
+    {  split; [|assumption].
+      apply VLSM_incl_finite_protocol_trace_from with (machine XE); [apply equivocators_limited_equivocations_vlsm_incl_free|].
+      assumption.
+    }
+    assert
+      (Htr'pre : finite_protocol_trace (pre_loaded_with_all_messages_vlsm FreeE) is tr').
+    { split; [|assumption].
+      specialize (vlsm_incl_pre_loaded_with_all_messages_vlsm FreeE) as Hincl.
+      apply (VLSM_incl_finite_protocol_trace_from _ _ Hincl). apply Htr'.
+    }
+    specialize
+      (equivocators_trace_project_preserves_proper_equivocator_descriptors _ _ (proj1 Htr'pre) _ _ _ Htr_project Hproper')
+      as Hproper_initial.
+    destruct oitem as [item|].
+    +  simpl in Hitemx. destruct Hitemx as [Hl [Hinput [Houtput Hdestination]]].
+      specialize (Hx _ eq_refl).
+      destruct Hx as [Hvx Htx].
+      exists (trX' ++ [item]), initial_descriptors. subst foldx.
+      rewrite equivocators_trace_project_folder_additive with (trX := trX') (eqv_descriptors := initial_descriptors)
+      ; [|assumption].
+      split; [assumption|].
+      split; [reflexivity|].
+      rewrite finite_trace_last_is_last.
+      unfold final_state. subst tr.
+      rewrite finite_trace_last_is_last.
+      split; [assumption|].
+      destruct HtrX' as [HtrX' His].
+      split; [|assumption].
+      apply finite_protocol_trace_from_app_iff.
+      split; [assumption|].
+      change [item] with ([] ++ [item]).
+      match goal with
+      |- finite_protocol_trace_from _ ?l _ => remember l as lst
+      end.
+      destruct item.
+      assert (Hplst : protocol_state_prop X' lst).
+      { apply finite_ptrace_last_pstate in HtrX'. subst. assumption. }
+      apply (extend_right_finite_trace_from X'); [constructor; assumption|].
+      simpl in Hl. subst.
+      simpl in Hc.
+      destruct Hc as [Hfull [[Hno_equiv _] Hlimited]].
+      simpl in Htx,Hvx,Hstate_project.
+      rewrite Hstate_project in Hvx, Htx.
+      destruct input as [input|]
+      ; [|repeat split; [assumption| apply option_protocol_message_None |assumption| apply HconstraintNone; assumption |assumption]]. 
+      simpl in Hno_equiv.
+      apply or_comm in Hno_equiv.
+      destruct Hno_equiv as [Hinit_input | Hno_equiv]
+      ; [apply fixed_equivocators_initial_message in Hinit_input|]
+      ; [repeat split; [assumption| |assumption| apply Hconstraintinitial; assumption |assumption]|].
+      { apply protocol_message_prop_iff. left. exists (exist _ _ Hinit_input).
+        reflexivity.
+      }
+      assert
+        (Hs_free : protocol_state_prop FreeE (finite_trace_last is tr')).
+      { destruct Hs as [_om Hs].
+        apply (constraint_subsumption_protocol_prop (equivocator_IM IM))
+          with (constraint2 := free_constraint (equivocator_IM IM))
+          in Hs as Hs_free
+          ; [|intro x; intros; exact I].
+        exists _om. assumption.
+      }
+      specialize
+        (specialized_proper_sent_rev FreeE _ Hs_free _ Hno_equiv) as Hall.
+      specialize (Hall is tr').
+      spec Hall (ptrace_add_default_last Htr').
+      destruct (equivocators_trace_project_output_reflecting_inv IM _ _ (proj1 Htr'pre) _ Hall)
+        as [final_descriptors_m [initial_descriptors_m [trXm [_Hfinal_descriptors_m [Hproject_trXm Hex]]]]].
+      assert (Hfinal_descriptors_m : proper_equivocator_descriptors IM final_descriptors_m (last (map Common.destination tr') is)).
+      { apply not_equivocating_equivocatos_descriptors_proper; [|assumption].
+        apply finite_ptrace_last_pstate. assumption.
+      }
+      specialize (H (length tr')).
+      spec H. { rewrite app_length. simpl. lia. }
+      specialize (H tr' (conj Htr Hinit) eq_refl final_descriptors_m Hfinal_descriptors_m).
+      destruct H as [trXm' [initial_descriptors_m' [Hproper_initial_m [Hproject_trXm' [Hpr_fin_tr' HtrXm]]]]].
+      simpl in *. rewrite Hproject_trXm in Hproject_trXm'.
+      inversion Hproject_trXm'. subst trXm' initial_descriptors_m'. clear Hproject_trXm'.
+      repeat split; [assumption| |assumption| |assumption]
+      ; [ apply option_protocol_message_Some
+        ; apply (protocol_trace_output_is_protocol X' _ _ (proj1 HtrXm) _ Hex)
+        |].
+      rewrite <- Hstate_project.
+      apply Hconstraint_hbs; [assumption| apply Hproper'|].
+      assert (Hlst'pre : protocol_state_prop (pre_loaded_with_all_messages_vlsm FreeE) (last (map Common.destination tr') is)).
+      { apply finite_ptrace_last_pstate. apply Htr'pre. }
+      apply proper_sent; [assumption|].
+      apply has_been_sent_consistency; [assumption| assumption| ].
+      exists is, tr', (ptrace_add_default_last Htr'pre). assumption.
+    + exists trX'. exists initial_descriptors. subst foldx. split; [assumption|].
+      split; [apply Htr_project|]. split; [|assumption].
+      subst tr. clear -Hstate_project Hx.
+      rewrite Hstate_project in Hx.
+      rewrite <- Hx. f_equal. unfold final_state.
+      rewrite finite_trace_last_is_last.
+      reflexivity.
+Qed.
+
+(** Instantiating the lemma above with the free constraint.
+*)
+Lemma free_equivocators_protocol_trace_project
+  (final_descriptors : equivocator_descriptors IM)
+  (is : composite_state (equivocator_IM IM))
+  (tr : list (composite_transition_item (equivocator_IM IM)))
+  (final_state := @finite_trace_last _ (@type _ XE) is tr)
+  (Hproper : proper_equivocator_descriptors IM final_descriptors final_state)
+  (Htr : finite_protocol_trace XE is tr)
+  : exists
+    (trX : list (composite_transition_item IM))
+    (initial_descriptors : equivocator_descriptors IM)
+    (isX := equivocators_state_project IM initial_descriptors is)
+    (final_stateX := finite_trace_last isX trX),
+    proper_equivocator_descriptors IM initial_descriptors is /\
+    equivocators_trace_project IM final_descriptors tr = Some (trX, initial_descriptors) /\
+    equivocators_state_project IM final_descriptors final_state = final_stateX /\
+    finite_protocol_trace (free_composite_vlsm IM) isX trX.
+Proof.
+  apply _equivocators_protocol_trace_project; [assumption | assumption| ..]
+  ; unfold constraint_has_been_sent_prop; intros; exact I.
+Qed.
+
+
+(**
+Main result of this section, stating that traces which are protocol for the
+equivocator-based definition of limited equivocation project to traces which are
+protocol for the simple-nodes definition of limited equivocation.
+*)
+Theorem limited_equivocators_protocol_trace_project
+  (final_descriptors : equivocator_descriptors IM)
+  (is : composite_state (equivocator_IM IM))
+  (tr : list (composite_transition_item (equivocator_IM IM)))
+  (final_state := finite_trace_last is tr)
+  (Hproper: proper_equivocator_descriptors IM final_descriptors final_state)
+  (Htr : finite_protocol_trace XE is tr)
+  : exists
+    (trX : list (composite_transition_item IM))
+    (initial_descriptors : equivocator_descriptors IM)
+    (isX := equivocators_state_project IM initial_descriptors is)
+    (final_stateX := finite_trace_last isX trX),
+    proper_equivocator_descriptors IM initial_descriptors is /\
+    equivocators_trace_project IM final_descriptors tr = Some (trX, initial_descriptors) /\
+    equivocators_state_project IM final_descriptors final_state = final_stateX /\
+    finite_protocol_trace X isX trX.
+Proof.
+  apply _equivocators_protocol_trace_project; [assumption | assumption| ..]
+  ; intros.
+  - split; [exact I|].
+    destruct (composite_transition IM l (s, None)) as (s', om') eqn:Ht.
+    rewrite
+      (@composite_transition_None_equivocators_weight
+        _ _ _ _ finite_index _ IM Hbs Hbr i0 sender globally_known_equivocators
+        Hdm Hknown_equivocators _ _ _ _ Ht
+      ).
+    apply
+      (full_node_limited_equivocation_protocol_state_weight
+        finite_index IM Hbs Hbr i0 sender globally_known_equivocators
+        _ H
+      ).
+  - split.
+    + destruct l. simpl.
+      intros dm Hdmm. 
+      rewrite
+        (initial_message_not_dependent sender (fun x => x) IM Hbs Hbr m H0)
+        in Hdmm.
+      inversion Hdmm.
+    + destruct (composite_transition IM l (s, Some m)) as (s', oom) eqn:Ht.
+      specialize
+        (known_equivocators_transition_no_equiv
+          finite_index IM Hbs Hbr i0 sender globally_known_equivocators
+          l s (Some m) s' oom Ht
+        ) as Hs'.
+      spec Hs'. { simpl. right. assumption. }
+      unfold globally_known_equivocators_weight.
+      specialize
+        (full_node_limited_equivocation_protocol_state_weight
+          finite_index IM Hbs Hbr i0 sender globally_known_equivocators
+          _ H
+        ) as Hs.
+      rewrite
+        (set_eq_nodup_sum_weight_eq
+          (globally_known_equivocators s')
+          (globally_known_equivocators s)
+        )
+      ; [assumption| .. | assumption]
+      ; apply
+          (known_equivocators_nodup
+            finite_index IM Hbs Hbr i0 sender globally_known_equivocators
+          ).
+  - intros s Hs descriptors Hdescriptors sX m Hmbs l.
+Admitted.
+
+
+
+
+End limited_equivocation_state_to_message.
